wip trying to prove [rsDown_atomic_messages_indep]

src/RqRsInvAtomic.v
@@ -2,80 +2,162 @@ Require Import Peano_dec Omega List ListSupport.
 Require Import Common FMap.
 Require Import Syntax Semantics SemFacts StepM Invariant Serial.
 Require Import Reduction Commutativity QuasiSeq Topology.
-Require Import RqRsTopo RqRsFacts.
+Require Import RqRsTopo RqRsFacts RqRsInvMsg.
 
 Set Implicit Arguments.
 
 Open Scope list.
 Open Scope fmap.
 
-(* Inductive TrsType := RqUp | RqDown | RsUp | RsDown. *)
-(* Object index -> TrsTypes (ordered, head is the oldest one) *)
-(* Definition TrsState := M.t (list TrsType). *)
+Definition lastOIdxOf (hst: MHistory): option IdxT :=
+  match hst with
+  | RlblInt oidx _ _ _ :: _ => Some oidx
+  | _ => None
+  end.
 
-(* Definition addTrsState (oidx: IdxT) (tr: TrsType) (ts: TrsState): TrsState := *)
-(*   match ts@[oidx] with *)
-(*   | Some tts => ts +[oidx <- tr :: tts] *)
-(*   | None => ts +[oidx <- [tr]] *)
-(*   end. *)
+Definition oidxOf (lbl: MLabel) :=
+  match lbl with
+  | RlblInt oidx _ _ _ => Some oidx
+  | _ => None
+  end.
 
-(* Definition rssOfL (lbl: MLabel) := *)
-(*   match lbl with *)
-(*   | RlblInt oidx _ _ mouts => *)
-(*     match mouts with *)
-(*     | nil => Some oidx (* Requests are never ignored. *) *)
-(*     | (midx, mout) :: _ => *)
-(*       if eq_nat_dec (msg_type mout) MRs *)
-(*       then Some oidx else None *)
-(*     end *)
-(*   | _ => None *)
-(*   end. *)
+Fixpoint oindsOf (hst: MHistory) :=
+  match hst with
+  | nil => nil
+  | lbl :: hst' => (oidxOf lbl) ::> (oindsOf hst')
+  end.
 
-(* Fixpoint rssOf (hst: MHistory): list IdxT := *)
-(*   match hst with *)
-(*   | nil => nil *)
-(*   | lbl :: hst' => (rssOfL lbl) ::> (rssOf hst') *)
-(*   end. *)
+Lemma atomic_lastOIdxOf:
+  forall inits ins hst outs eouts,
+    Atomic msg_dec inits ins hst outs eouts ->
+    exists loidx,
+      lastOIdxOf hst = Some loidx.
+Proof.
+  induction 1; simpl; intros; eauto.
+Qed.
 
-(* Section AtomicInv. *)
-(*   Context {oifc: OStateIfc}. *)
-(*   Variables (dtr: DTree) *)
-(*             (sys: System oifc). *)
+Section RqUpPrefix.
+  Context {oifc: OStateIfc}.
+  Variables (dtr: DTree)
+            (sys: System oifc).
 
-(*   Hypothesis (Hitr: GoodRqRsSys dtr sys). *)
+  Hypothesis (Hrrs: RqRsSys dtr sys).
 
-(*   Definition rsUpCover (idm: Id Msg): list IdxT := *)
-(*     nil. (** TODO: define it. *) *)
-
-(*   Fixpoint rsUpCovers (eouts: list (Id Msg)): list IdxT := *)
-(*     match eouts with *)
-(*     | nil => nil *)
-(*     | idm :: eouts' => rsUpCover idm ++ rsUpCovers eouts' *)
-(*     end. *)
-
-(*   Definition rsDownCover (idm: Id Msg): list IdxT := *)
-(*     nil. (** TODO: define it. *) *)
-
-(*   Fixpoint rsDownCovers (eouts: list (Id Msg)): list IdxT := *)
-(*     match eouts with *)
-(*     | nil => nil *)
-(*     | idm :: eouts' => rsDownCover idm ++ rsDownCovers eouts' *)
-(*     end. *)
-
-(*   Definition AtomicInv (inits eouts: list (Id Msg)) (hst: MHistory) := *)
-(*     NoDup (rssOf hst) /\ *)
-(*     SubList (rssOf hst) (rsUpCovers eouts) /\ *)
-(*     DisjList (rssOf hst) (rsDownCovers eouts). *)
-
-(*   Lemma atomic_inv: *)
-(*     forall inits ins hst outs eouts, *)
-(*       Atomic msg_dec inits ins hst outs eouts -> *)
-(*       forall s1 s2, *)
-(*         steps step_m sys s1 hst s2 -> *)
-(*         AtomicInv inits eouts hst. *)
-(*   Proof. *)
+  (* Inductive RqUpPrefix: *)
+  (*   MHistory (* hst *) -> *)
+  (*   MHistory (* RqUp prefix of [hst] *) -> *)
+  (*   option IdxT (* The most recent RqUp queue index, if growing *) -> *)
+  (*   Prop := *)
+  (* | RqUpPrefixRs: *)
+  (*     forall cidx oidx ridx ruFrom ruTo rufm rutm, *)
+  (*       parentIdxOf dtr cidx = Some oidx -> *)
+  (*       rqEdgeUpFrom dtr cidx = Some ruFrom -> *)
+  (*       rqEdgeUpFrom dtr oidx = Some ruTo -> *)
+  (*       RqUpPrefix [RlblInt ridx oidx [(ruFrom, rufm)] [(ruTo, rutm)]] *)
+  (*                  [RlblInt ridx oidx [(ruFrom, rufm)] [(ruTo, rutm)]] (Some ruTo) *)
+  (* | RqUpPrefixRc: *)
+  (*     forall hst cidx oidx ridx rus ruFrom ruTo rufm rutm, *)
+  (*       RqUpPrefix hst rus (Some ruFrom) -> *)
+  (*       parentIdxOf dtr cidx = Some oidx -> *)
+  (*       rqEdgeUpFrom dtr cidx = Some ruFrom -> *)
+  (*       rqEdgeUpFrom dtr oidx = Some ruTo -> *)
+  (*       RqUpPrefix (RlblInt ridx oidx [(ruFrom, rufm)] [(ruTo, rutm)] :: hst) *)
+  (*                  (RlblInt ridx oidx [(ruFrom, rufm)] [(ruTo, rutm)] :: rus) *)
+  (*                  (Some ruTo) *)
   
-(* End AtomicInv. *)
+  (* Lemma atomic_RqUpHistory_prefix: *)
+  (*   forall inits ins hst outs eouts, *)
+  (*     Atomic msg_dec inits ins hst outs eouts -> *)
+  (*     forall s1 s2, *)
+  (*       Reachable (steps step_m) sys s1 -> *)
+  (*       steps step_m sys s1 hst s2 -> *)
+  (*       exists phst nhst, *)
+  (*         hst = nhst ++ phst /\ *)
+  (*         (phst = nil \/ *)
+  (*          exists pins pouts rqUps ruIdx, *)
+  (*            Atomic msg_dec inits pins phst pouts rqUps /\ *)
+  (*            RqUpMsgs dtr ruIdx rqUps /\ *)
+  (*            RqUpHistory dtr phst rqUps /\ *)
+  (*            (nhst = nil \/ *)
+  (*             exists noidx nridx nrouts nrhst nins nouts, *)
+  (*               nhst = nrhst ++ [RlblInt noidx nridx rqUps nrouts] /\ *)
+  (*               Atomic msg_dec rqUps nins nhst nouts eouts /\ *)
+                
+  (* Proof. *)
+  (*   induction 1; simpl; intros; subst. *)
+  (*   - admit. *)
+
+  (*   - inv_steps. *)
+  (*     specialize (IHAtomic _ _ H5 H7). *)
+  (*     destruct IHAtomic as [phst [nhst ?]]; dest; subst. *)
+
+End RqUpPrefix.
+
+Section Covers.
+  Context {oifc: OStateIfc}.
+  Variables (dtr: DTree)
+            (sys: System oifc).
+
+  Hypothesis (Hrrs: RqRsSys dtr sys).
+
+  Definition RqUpCoverInv (oinds: list IdxT) (rqUp: Id Msg) :=
+    forall ruFrom ruTo,
+      msg_type (valOf rqUp) = MRq ->
+      parentIdxOf dtr ruFrom = Some ruTo ->
+      rqEdgeUpFrom dtr ruFrom = Some (idOf rqUp) ->
+      SubList oinds (subtreeIndsOf dtr ruFrom).
+
+  Definition RqDownCoverInv (oinds: list IdxT) (rqDown: Id Msg) :=
+    forall rdFrom rdTo,
+      msg_type (valOf rqDown) = MRq ->
+      parentIdxOf dtr rdTo = Some rdFrom ->
+      edgeDownTo dtr rdTo = Some (idOf rqDown) ->
+      DisjList oinds (subtreeIndsOf dtr rdTo).
+
+  Definition RsUpCoverInv (oinds: list IdxT) (rsUp: Id Msg) :=
+    True.
+
+  Definition RsDownCoverInv (oinds: list IdxT) (rsDown: Id Msg) :=
+    forall rdFrom rdTo,
+      msg_type (valOf rsDown) = MRs ->
+      parentIdxOf dtr rdTo = Some rdFrom ->
+      edgeDownTo dtr rdTo = Some (idOf rsDown) ->
+      DisjList oinds (subtreeIndsOf dtr rdTo).
+
+  Definition CoverInvMsg (oinds: list IdxT) (eout: Id Msg) :=
+    RqUpCoverInv oinds eout /\
+    RqDownCoverInv oinds eout /\
+    RsUpCoverInv oinds eout.
+
+  Definition CoverInv (oinds: list IdxT) (eouts: list (Id Msg)) :=
+    Forall (CoverInvMsg oinds) eouts.
+
+  Ltac disc_rule_custom ::=
+    try disc_footprints_ok.
+  
+  (* Lemma cover_inv: *)
+  (*   forall inits ins hst outs eouts, *)
+  (*     Atomic msg_dec inits ins hst outs eouts -> *)
+  (*     forall s1 s2, *)
+  (*       Reachable (steps step_m) sys s1 -> *)
+  (*       steps step_m sys s1 hst s2 -> *)
+  (*       CoverInv (oindsOf hst) eouts. *)
+  (* Proof. *)
+  (*   destruct Hrrs as [? [? ?]]. *)
+  (*   induction 1; simpl; intros. *)
+
+  (*   - inv_steps; inv_step. *)
+  (*     admit. *)
+  (*     (* good_rqrs_rule_get rule. *) *)
+  (*     (* good_rqrs_rule_cases rule. *) *)
+
+
+  (*   - inv_steps; inv_step. *)
+      
+
+          
+  
+End Covers.
 
 Close Scope list.
 Close Scope fmap.
