src/RqRsInvUpLock.v
@@ -2306,6 +2306,46 @@ Section UpLockInv.
   
 End UpLockInv.
 
+Lemma upLockInvORq_rqUp_length_two_False:
+  forall dtr orqs msgs oidx orq pidx rqUp,
+    UpLockInvORq dtr orqs msgs oidx orq ->
+    parentIdxOf dtr oidx = Some pidx ->
+    rqEdgeUpFrom dtr oidx = Some rqUp ->
+    length (findQ rqUp msgs) >= 2 ->
+    False.
+Proof.
+  intros.
+  red in H; destruct (orq@[upRq]).
+  - destruct H as [rrqUp [down [rpidx ?]]]; dest.
+    repeat disc_rule_minds.
+    omega.
+  - destruct H.
+    + congruence.
+    + destruct H as [rrqUp [down [rpidx ?]]]; dest.
+      repeat disc_rule_minds.
+      rewrite H5 in H2; simpl in H2; omega.
+Qed.
+
+Lemma upLockInvORq_down_rssQ_length_two_False:
+  forall dtr orqs msgs oidx orq pidx down,
+    UpLockInvORq dtr orqs msgs oidx orq ->
+    parentIdxOf dtr oidx = Some pidx ->
+    edgeDownTo dtr oidx = Some down ->
+    length (rssQ msgs down) >= 2 ->
+    False.
+Proof.
+  intros.
+  red in H; destruct (orq@[upRq]).
+  - destruct H as [rqUp [rdown [rpidx ?]]]; dest.
+    repeat disc_rule_minds.
+    omega.
+  - destruct H.
+    + congruence.
+    + destruct H as [rqUp [rdown [rpidx ?]]]; dest.
+      repeat disc_rule_minds.
+      rewrite H6 in H2; simpl in H2; omega.
+Qed.
+
 Close Scope list.
 Close Scope fmap.
 
